src/crypto/aes/AES_s.fst
@@ -98,19 +98,4 @@ let key_to_round_keys (alg:algorithm) (key:aes_key alg)
 let aes_encrypt (alg:algorithm) (key:aes_key alg) (input:quad32) =
   cipher alg input (key_to_round_keys alg key)
 
-#reset-options "--max_fuel 5 --initial_fuel 5"
-abstract let quad32_to_seq (q:quad32) : 
-  Tot (s:seq nat32 { length s == 4 /\ 
-                     (let q' = Quad32 (index s 0) (index s 1) (index s 2) (index s 3) in
-                      q == q')           
-                   }) =
-  let l = [q.lo; q.mid_lo; q.mid_hi; q.hi] in
-  let s = of_list l in
-  //assert (List.length l == 4);
-  lemma_of_list_length s l; 
-  lemma_of_list s l 0;
-  lemma_of_list s l 1;
-  lemma_of_list s l 2;
-  lemma_of_list s l 3;  
-  of_list l
 
